Add task defs, fast equality for all hashconsed types

extract/TaskExtra.ml
@@ -1,0 +1,390 @@
+(********************************************************************)
+(*                                                                  *)
+(*  The Why3 Verification Platform   /   The Why3 Development Team  *)
+(*  Copyright 2010-2023 --  Inria - CNRS - Paris-Saclay University  *)
+(*                                                                  *)
+(*  This software is distributed under the terms of the GNU Lesser  *)
+(*  General Public License version 2.1, with the special exception  *)
+(*  on linking described in file LICENSE.                           *)
+(*                                                                  *)
+(********************************************************************)
+
+open Ident
+open Ty
+open Term
+open Decl
+(* open Theory *)
+
+(** Clone and meta history *)
+
+(*Trying to switch see*)
+(* module Stdecl = Theory.Stdecl1 *)
+
+let stdecl_id (s: Stdecl1.t) : BigInt.t =
+  Stdecl1.fold (fun t acc -> Hashcons.combine_big t.td_tag acc) s (BigInt.of_int 3)
+
+(* module Stdecl = Hcpt.MakeSet(struct
+  type t = tdecl
+  let id td = BigInt.to_int td.td_tag 
+end) *)
+(* module HStdecl = Stdecl *)
+
+(* type tdecl_set = Stdecl.t *)
+
+module Wtds = Weakhtbl.Make(struct
+  type t = tdecl_set
+  let tag s = Weakhtbl.create_tag (stdecl_id s) (*(Stdecl.id s)*)
+  let equal = (==) (*JOSH TODO equal*)
+end)
+
+
+let mk_tds s =
+  Theory.Stdecl.fold Stdecl.add s Stdecl.empty
+
+let tds_empty = Stdecl.empty
+let tds_singleton td = Stdecl.singleton td
+
+let tds_add = Stdecl.add
+
+let tds_equal = Stdecl.equal
+(* let tds_hash = Stdecl.hash 
+JOSH SEE *)
+let tds_compare = Stdecl.compare
+
+(* type clone_map = tdecl_set Mid.t
+type meta_map = tdecl_set Mmeta.t *)
+
+let cm_find cm th = Mid.find_def tds_empty th.th_name cm
+let mm_find mm t = Mmeta.find_def tds_empty t mm
+
+let cm_add cm th td = Mid.change (function
+  | None -> Some (tds_singleton td)
+  | Some tds -> Some (tds_add td tds)) th.th_name cm
+
+let mm_add mm t td = Mmeta.change (function
+  | None -> Some (tds_singleton td)
+  | Some tds -> Some (tds_add td tds)) t mm
+
+let mm_add mm t td = if t.meta_excl
+  then Mmeta.add t (tds_singleton td) mm
+  else mm_add mm t td
+
+(** Task *)
+
+(* type task = task_hd option
+
+and task_hd = {
+  task_decl  : tdecl;        (* last declaration *)
+  task_prev  : task;         (* context *)
+  task_known : known_map;    (* known identifiers *)
+  task_clone : clone_map;    (* use/clone history *)
+  task_meta  : meta_map;     (* meta properties *)
+  task_tag   : Weakhtbl.tag; (* unique magical tag *)
+} *)
+
+(* let task_hd_equal t1 t2 = match t1.task_decl.td_node, t2.task_decl.td_node with
+  | Decl {d_node = Dprop (Pgoal,p1,g1)}, Decl {d_node = Dprop (Pgoal,p2,g2)} ->
+      Option.equal (==) t1.task_prev t2.task_prev &&
+      pr_equal p1 p2 && t_equal_strict g1 g2
+  | _ -> t1 == t2
+
+let task_hd_hash t = Weakhtbl.tag_hash t.task_tag
+
+let task_equal t1 t2 = Option.equal task_hd_equal t1 t2
+
+let task_hash t = Option.fold ~some:(fun t -> BigInt.succ (task_hd_hash t)) ~none:BigInt.zero t *)
+
+(* module Hstask = Hashcons.Make (struct
+  type t = task_hd
+
+  let equal t1 t2 = td_equal t1.task_decl t2.task_decl &&
+                  task_equal t1.task_prev t2.task_prev
+
+  let hash t =  (Hashcons.combine_big (td_hash t.task_decl) (task_hash t.task_prev))
+
+  let tag i task = { task with task_tag = Weakhtbl.create_tag i }
+end)
+
+let mk_task decl prev known clone meta = Some (Hstask.hashcons {
+  task_decl  = decl;
+  task_prev  = prev;
+  task_known = known;
+  task_clone = clone;
+  task_meta  = meta;
+  task_tag   = Weakhtbl.dummy_tag;
+}) *)
+
+let task_known o = Option.fold ~some:(fun t -> t.task_known) ~none:Mid.empty   o
+let task_clone o = Option.fold ~some:(fun t -> t.task_clone) ~none:Mid.empty   o
+let task_meta  o = Option.fold ~some:(fun t -> t.task_meta)  ~none:Mmeta.empty o
+
+let find_clone_tds task (th : theory) = cm_find (task_clone task) th
+let find_meta_tds task (t : meta) = mm_find (task_meta task) t
+
+(* constructors with checks *)
+
+exception LemmaFound
+exception GoalFound
+exception GoalNotFound
+
+let find_goal = function
+  | Some {task_decl = {td_node = Decl {d_node = Dprop (Pgoal,p,f)}}} ->
+      Some(p,f)
+  | _ -> None
+
+let task_goal task = match find_goal task with
+  | Some (pr,_) -> pr
+  | None        -> raise GoalNotFound
+
+let task_goal_fmla task  = match find_goal task with
+  | Some (_,f)  -> f
+  | None        -> raise GoalNotFound
+
+let task_separate_goal = function
+  | Some {task_decl = {td_node = Decl {d_node = Dprop (Pgoal,_,_)}} as goal;
+          task_prev = task} ->
+      goal,task
+  | _ -> raise GoalNotFound
+
+let check_task task = match find_goal task with
+  | Some _  -> raise GoalFound
+  | None    -> task
+
+let check_decl = function
+  | {d_node = Dprop (Plemma,_,_)} -> raise LemmaFound
+  | d -> d
+
+let new_decl task d td =
+  let (d1, kn) = known_add_decl (task_known task) (check_decl d) in
+  let td1 = create_decl d1 in
+  mk_task td1 (check_task task) kn (task_clone task) (task_meta task)
+
+let new_decl task d td = try new_decl task d td with KnownIdent _ -> task
+
+let new_clone task th td =
+  let cl = cm_add (task_clone task) th td in
+  mk_task td (check_task task) (task_known task) cl (task_meta task)
+
+let new_meta task t td =
+  let mt = mm_add (task_meta task) t td in
+  mk_task td (check_task task) (task_known task) (task_clone task) mt
+
+(* declaration constructors + add_decl *)
+
+let add_decl task d = new_decl task d (create_decl d)
+
+let add_ty_decl tk ts = add_decl tk (create_ty_decl ts)
+let add_data_decl tk dl = add_decl tk (create_data_decl dl)
+let add_param_decl tk ls = add_decl tk (create_param_decl ls)
+let add_logic_decl tk dl = add_decl tk (create_logic_decl dl)
+let add_ind_decl tk s dl = add_decl tk (create_ind_decl s dl)
+let add_prop_decl tk k p f = add_decl tk (create_prop_decl k p f)
+
+(* task constructors *)
+
+let add_tdecl task td = match td.td_node with
+  | Decl d -> new_decl task d td
+  | Use th ->
+      if Stdecl.mem td (find_clone_tds task th) then task else
+      new_clone task th td
+  | Clone (th,_) -> new_clone task th td
+  | Meta (t,_) -> new_meta task t td
+
+let rec flat_tdecl task td = match td.td_node with
+  | Decl { d_node = Dprop (Plemma,pr,f) } -> add_prop_decl task Paxiom pr f
+  | Decl { d_node = Dprop (Pgoal,_,_) } -> task
+  | Decl d -> new_decl task d td
+  | Use th -> use_export task th td
+  | Clone (th,_) -> new_clone task th td
+  | Meta (t,_) -> new_meta task t td
+
+and use_export task th td =
+  if Stdecl.mem td (find_clone_tds task th) then task else
+  let task = List.fold_left flat_tdecl task th.th_decls in
+  new_clone task th td
+
+let use_export task th = use_export task th (create_use th)
+
+let clone_export = clone_theory flat_tdecl
+
+let add_meta task t al = new_meta task t (create_meta t al)
+
+(* split theory *)
+
+let theory_goals th names =
+  if Opt.fold (fun _ s -> Spr.is_empty s) false names then Spr.empty else
+  let named pr = match names with Some gs -> Spr.mem pr gs | _ -> true in
+  let collect prs td = match td.td_node with
+    | Clone (th, sm) -> (* do not reprove instantiations of lemmas *)
+        Mpr.fold (fun o n prs -> match find_prop_decl th.th_known o with
+          | (Plemma|Pgoal),_ -> Spr.remove n prs | _ -> prs) sm.sm_pr prs
+    | Decl { d_node = Dprop ((Plemma|Pgoal),pr,_) } when named pr ->
+        Spr.add pr prs
+    | _ -> prs in
+  List.fold_left collect Spr.empty th.th_decls
+
+let split_theory th names init =
+  let prs = theory_goals th names in
+  if Spr.is_empty prs then [] else
+  let split (task, acc) td = flat_tdecl task td, match td.td_node with
+    | Decl { d_node = Dprop ((Plemma|Pgoal),pr,f) } when Spr.mem pr prs ->
+        add_prop_decl task Pgoal pr f :: acc
+    | _ -> acc in
+  List.rev (snd (List.fold_left split (init, []) th.th_decls))
+
+(* Generic utilities *)
+
+let rec task_fold fn acc = function
+  | Some task -> task_fold fn (fn acc task.task_decl) task.task_prev
+  | None      -> acc
+
+let rec task_iter fn = function
+  | Some task -> fn task.task_decl; task_iter fn task.task_prev
+  | None      -> ()
+
+let task_tdecls = task_fold (fun acc td -> td::acc) []
+
+let task_decls  = task_fold (fun acc td ->
+  match td.td_node with Decl d -> d::acc | _ -> acc) []
+
+(* Realization utilities *)
+
+let check_use td = match td.td_node with
+  | Use _ -> true
+  | Clone _ -> false
+  | _ -> assert false
+
+let used_theories task =
+  let used s =
+    let th = match (Stdecl.choose s).td_node with
+      | Use th
+      | Clone (th, _) -> th
+      | _ -> assert false
+    in
+    if Stdecl.exists_ check_use s then Some th else None
+  in
+  Mid.map_filter used (task_clone task)
+
+let used_symbols thmap =
+  let dict th = Mid.map (fun () -> th) th.th_local in
+  let join _ = Mid.union (fun _ -> assert false) in
+  Mid.fold join (Mid.map dict thmap) Mid.empty
+
+let local_decls task symbmap =
+  let rec skip t = function
+    | { td_node = Use th } :: rest
+      when id_equal t.th_name th.th_name -> rest
+    | _ :: rest -> skip t rest
+    | [] -> []
+  in
+  let rec filter acc = function
+    | { td_node = Decl d } :: rest ->
+        let id = Sid.choose d.d_news in
+        (try filter acc (skip (Mid.find id symbmap) rest)
+        with Not_found -> filter (d::acc) rest)
+    | _ :: rest -> filter acc rest
+    | [] -> List.rev acc
+  in
+  filter [] (task_tdecls task)
+
+(* Selectors *)
+
+exception NotTaggingMeta of meta
+exception NotExclusiveMeta of meta
+
+let on_meta t fn acc task =
+  let add td acc = match td.td_node with
+    | Meta (_,ma) -> fn acc ma
+    | _ -> assert false
+  in
+  let tds = find_meta_tds task t in
+  Stdecl.fold add tds acc
+
+let on_cloned_theory th fn acc task =
+  let add td acc = match td.td_node with
+    | Clone (_,sm) -> fn acc sm
+    | Use _ -> acc
+    | _ -> assert false
+  in
+  let tds = find_clone_tds task th in
+  Stdecl.fold add tds acc
+
+let on_meta_excl t task =
+  if not t.meta_excl then raise (NotExclusiveMeta t);
+  let add td _ = match td.td_node with
+    | Meta (_,ma) -> Some ma
+    | _ -> assert false
+  in
+  let tds = find_meta_tds task t in
+  Stdecl.fold add tds None
+
+let on_used_theory th task =
+  let tds = find_clone_tds task th in
+  Stdecl.exists_ check_use tds
+
+let on_tagged_ty t task =
+  begin match t.meta_type with
+    | MTty :: _ -> ()
+    | _ -> raise (NotTaggingMeta t)
+  end;
+  let add td acc = match td.td_node with
+    | Meta (_, MAty ty :: _) -> Sty.add ty acc
+    | _ -> assert false
+  in
+  let tds = find_meta_tds task t in
+  Stdecl.fold add tds Sty.empty
+
+let on_tagged_ts t task =
+  begin match t.meta_type with
+    | MTtysymbol :: _ -> ()
+    | _ -> raise (NotTaggingMeta t)
+  end;
+  let add td acc = match td.td_node with
+    | Meta (_, MAts ts :: _) -> Sts.add ts acc
+    | _ -> assert false
+  in
+  let tds = find_meta_tds task t in
+  Stdecl.fold add tds Sts.empty
+
+let on_tagged_ls t task =
+  begin match t.meta_type with
+    | MTlsymbol :: _ -> ()
+    | _ -> raise (NotTaggingMeta t)
+  end;
+  let add td acc = match td.td_node with
+    | Meta (_, MAls ls :: _) -> Sls.add ls acc
+    | _ -> assert false
+  in
+  let tds = find_meta_tds task t in
+  Stdecl.fold add tds Sls.empty
+
+let on_tagged_pr t task =
+  begin match t.meta_type with
+    | MTprsymbol :: _ -> ()
+    | _ -> raise (NotTaggingMeta t)
+  end;
+  let add td acc = match td.td_node with
+    | Meta (_, MApr pr :: _) -> Spr.add pr acc
+    | _ -> assert false
+  in
+  let tds = find_meta_tds task t in
+  Stdecl.fold add tds Spr.empty
+
+
+(* Exception reporting *)
+
+let () = Exn_printer.register (fun fmt exn -> match exn with
+  | LemmaFound ->   Format.pp_print_string fmt "Task cannot contain a lemma"
+  | GoalFound ->    Format.pp_print_string fmt "The task already ends with a goal"
+  | GoalNotFound -> Format.pp_print_string fmt "The task does not end with a goal"
+  | NotTaggingMeta m ->
+      Format.fprintf fmt "Metaproperty '%s' is not a symbol tag" m.meta_name
+  | NotExclusiveMeta m ->
+      Format.fprintf fmt "Metaproperty '%s' is not exclusive" m.meta_name
+  | _ -> raise exn)
+
+(* task1 : prefix
+   lt : to reduce
+   lk : suffix (reverse order)
+   i : length of lt
+*)
