extract/task.mli
@@ -1,0 +1,143 @@
+(********************************************************************)
+(*                                                                  *)
+(*  The Why3 Verification Platform   /   The Why3 Development Team  *)
+(*  Copyright 2010-2023 --  Inria - CNRS - Paris-Saclay University  *)
+(*                                                                  *)
+(*  This software is distributed under the terms of the GNU Lesser  *)
+(*  General Public License version 2.1, with the special exception  *)
+(*  on linking described in file LICENSE.                           *)
+(*                                                                  *)
+(********************************************************************)
+
+(** Proof Tasks, Cloning and Meta History *)
+
+open Ident
+open Ty
+open Term
+open Decl
+open Theory
+
+module HStdecl = Theory.Stdecl1
+
+(* module HStdecl : Hcpt.S with type elt = tdecl *)
+
+type tdecl_set = HStdecl.t
+
+module Wtds: Weakhtbl.S with type key = tdecl_set
+
+val tds_equal : tdecl_set -> tdecl_set -> bool
+(* val tds_hash : tdecl_set -> int *)
+val tds_compare : tdecl_set -> tdecl_set -> int
+val tds_empty : tdecl_set
+
+val mk_tds : Stdecl.t -> tdecl_set
+
+type clone_map = tdecl_set Mid.t    (* Use and Clone *)
+type meta_map = tdecl_set Mmeta.t   (* Meta *)
+
+(** Task *)
+
+type task = task_hd option
+
+and task_hd = private {
+  task_decl  : tdecl;        (** last declaration *)
+  task_prev  : task;         (** context *)
+  task_known : known_map;    (** known identifiers *)
+  task_clone : clone_map;    (** use/clone history *)
+  task_meta  : meta_map;     (** meta properties *)
+  task_tag   : Weakhtbl.tag; (** unique magical tag *)
+}
+
+val task_equal : task -> task -> bool
+val task_hd_equal : task_hd -> task_hd -> bool
+
+val task_hash : task -> BigInt.t
+val task_hd_hash : task_hd -> BigInt.t
+
+val task_known : task -> known_map
+val task_clone : task -> clone_map
+val task_meta  : task -> meta_map
+
+val find_clone_tds : task -> theory -> tdecl_set
+val find_meta_tds  : task -> meta -> tdecl_set
+
+(** {2 Constructors} *)
+
+val add_decl : task -> decl -> task
+val add_tdecl : task -> tdecl -> task
+
+val use_export : task -> theory -> task
+val clone_export : task -> theory -> th_inst -> task
+val add_meta : task -> meta -> meta_arg list -> task
+
+(** {2 Declaration constructors + add_decl} *)
+
+val add_ty_decl : task -> tysymbol -> task
+val add_data_decl : task -> data_decl list -> task
+val add_param_decl : task -> lsymbol -> task
+val add_logic_decl : task -> logic_decl list -> task
+val add_ind_decl : task -> ind_sign -> ind_decl list -> task
+val add_prop_decl : task -> prop_kind -> prsymbol -> term -> task
+
+(** {2 Utilities} *)
+
+val split_theory : theory -> Spr.t option -> task -> task list
+  (** [split_theory th s t] returns the list of proof tasks that
+      correspond to goals in [th], in the order of appearance.
+      If set [s] is not empty, then only the goals in [s] are
+      proved. The goals which are instances of already proved
+      propositions (introduced by cloning) are not proved.
+      Task [t] is the task prefix that can be used to add
+      some metas to every generated proof task. *)
+
+(** {2 Realization utilities} *)
+
+val used_theories : task -> theory Mid.t
+  (** returns a map from theory names to theories themselves *)
+
+val used_symbols : theory Mid.t -> theory Mid.t
+  (** takes the result of {!used_theories} and returns
+      a map from symbol names to their theories of origin *)
+
+val local_decls : task -> theory Mid.t -> decl list
+  (** takes the result of {!used_symbols} and returns
+      the list of declarations that are not imported
+      with those theories or derived thereof *)
+
+(** {2 Bottom-up, tail-recursive traversal functions} *)
+
+val task_fold : ('a -> tdecl -> 'a) -> 'a -> task -> 'a
+val task_iter : (tdecl -> unit) -> task -> unit
+
+val task_tdecls : task -> tdecl list
+val task_decls  : task -> decl list
+
+val task_goal  : task -> prsymbol
+val task_goal_fmla  : task -> term
+
+val task_separate_goal : task -> tdecl * task
+(** [task_separate_goal t] returns a pair [(g,t')] where [g] is the
+    goal of the task [t] and [t'] is the rest.  Raises {!GoalNotFound}
+    if task [t] has no goal *)
+
+(** {2 Selectors} *)
+
+val on_meta : meta -> ('a -> meta_arg list -> 'a) -> 'a -> task -> 'a
+val on_cloned_theory : theory -> ('a -> symbol_map -> 'a) -> 'a -> task -> 'a
+
+val on_meta_excl : meta -> task -> meta_arg list option
+val on_used_theory : theory -> task -> bool
+
+val on_tagged_ty : meta -> task -> Sty.t
+val on_tagged_ts : meta -> task -> Sts.t
+val on_tagged_ls : meta -> task -> Sls.t
+val on_tagged_pr : meta -> task -> Spr.t
+
+(** Exceptions *)
+
+exception NotTaggingMeta of meta
+exception NotExclusiveMeta of meta
+
+exception GoalNotFound
+exception GoalFound
+exception LemmaFound
