src/core/TaskDefs.v
@@ -1,27 +1,122 @@
-Require Import DeclDefs DeclFuncs TheoryDefs.
+Require Import Monads PmapExtra CoqWeakhtbl IdentDefs TermFuncs DeclDefs DeclFuncs TheoryDefs.
+Import MonadNotations.
 
 (*Clone and Meta History*)
+Module Stdecl := TheoryDefs.Stdecl1.
+Module HStdecl := Stdecl.
+Definition tdecl_set := Stdecl.t.
+Definition clone_map := Mid.t tdecl_set.
+Definition meta_map := Mmeta.t tdecl_set.
 
-(* 
+
 (** Task *)
-Inductive task_head := mk_task_head {
-  task_decl  : tdecl;        (* last declaration *)
-  task_prev  : option task_head;         (* context *)
+Unset Elimination Schemes.
+Inductive task_hd := mk_task_head {
+  task_decl  : tdecl_c;        (* last declaration *)
+  task_prev  : option task_hd;         (* context *)
   task_known : known_map;    (* known identifiers *)
   task_clone : clone_map;    (* use/clone history *)
   task_meta  : meta_map;     (* meta properties *)
-  task_tag   : Weakhtbl.tag; (* unique magical tag *)
+  task_tag   : CoqWeakhtbl.tag; (* unique magical tag *)
 }.
+Set Elimination Schemes.
 
-Definition task := option task_head.
+Definition task := option task_hd.
 
-type task = task_hd option
+(*Induction and Decidable Equality*)
+Section TaskInd.
 
-and task_hd = {
-  task_decl  : tdecl;        (* last declaration *)
-  task_prev  : task;         (* context *)
-  task_known : known_map;    (* known identifiers *)
-  task_clone : clone_map;    (* use/clone history *)
-  task_meta  : meta_map;     (* meta properties *)
-  task_tag   : Weakhtbl.tag; (* unique magical tag *)
-} *)
+Variable (P: task_hd -> Prop).
+Variable (Hind: forall t, option_Forall P t.(task_prev) ->
+  P t).
+
+Fixpoint task_hd_ind (t: task_hd) : P t :=
+  Hind t (mk_option_Forall task_hd_ind t.(task_prev)).
+
+End TaskInd.
+
+Fixpoint task_hd_eqb (t1 t2: task_hd) : bool :=
+  CoqWeakhtbl.tag_equal t1.(task_tag) t2.(task_tag) && (*tag first*)
+  td_equal t1.(task_decl) t2.(task_decl) &&
+  option_eqb task_hd_eqb t1.(task_prev) t2.(task_prev) &&
+  Mid.equal d_equal t1.(task_known) t2.(task_known) &&
+  Mid.equal Stdecl.equal t1.(task_clone) t2.(task_clone) &&
+  Mmeta.equal Stdecl.equal t1.(task_meta) t2.(task_meta).
+
+Lemma task_hd_eqb_eq t1 t2:
+  t1 = t2 <-> task_hd_eqb t1 t2.
+Proof.
+  revert t2. apply task_hd_ind with (P:=fun t1 =>
+    forall t2, t1 = t2 <-> task_hd_eqb t1 t2); clear; intros t1 IH t2.
+  destruct t1; destruct t2; simpl in *.
+  rewrite !andb_true, <- tdecl_eqb_eq, <- (option_eqb_Forall IH),
+  <- (Mid.eqb_eq _ decl_eqb_eq ident_eqb_eq),
+  <- (Mid.eqb_eq _ (Stdecl.equal_eq tdecl_eqb_eq) ident_eqb_eq),
+  <- (Mmeta.eqb_eq _ (Stdecl.equal_eq tdecl_eqb_eq) meta_eqb_eq),
+  <- CoqWeakhtbl.tag_equal_eq.
+  solve_eqb_eq.
+Qed.
+
+Definition task_hd_eqb_fast := task_hd_eqb.
+
+
+(*Equality and Hashconsing*)
+
+Definition task_hd_equal (t1 t2: task_hd) : bool :=
+  match td_node_of t1.(task_decl), td_node_of t2.(task_decl) with
+  | Decl d1, Decl d2 =>
+    match d1.(d_node), d2.(d_node) with
+    | Dprop x1, Dprop x2 =>
+      let '(k1, p1, g1) := of_tup3 x1 in
+      let '(k2, p2, g2) := of_tup3 x2 in
+      match k1, k2 with
+      | Pgoal, Pgoal =>
+        option_eqb task_hd_eqb_fast t1.(task_prev) t2.(task_prev) &&
+        pr_equal p1 p2 && t_equal_strict g1 g2
+      | _, _ => task_hd_eqb_fast t1 t2
+      end
+    | _, _ => task_hd_eqb_fast t1 t2
+    end
+  | _, _ => task_hd_eqb_fast t1 t2
+  end.
+
+Definition task_hd_hash (t: task_hd) : CoqBigInt.t :=
+  CoqWeakhtbl.tag_hash t.(task_tag).
+
+Definition task_equal (t1 t2: task) : bool :=
+  option_eqb task_hd_eqb_fast t1 t2.
+
+Definition task_hash (t: task) : CoqBigInt.t :=
+  option_fold CoqBigInt.zero (fun t => CoqBigInt.succ (task_hd_hash t)) t.
+
+(*Hashconsing*)
+Module TaskHash <: hashcons.HashedType.
+Definition t := task_hd.
+Definition equal (t1 t2: t) : bool :=
+  td_equal t1.(task_decl) t2.(task_decl) &&
+  task_equal t1.(task_prev) t2.(task_prev).
+Definition hash (t1: t) : CoqBigInt.t :=
+  hashcons.combine_big (td_hash t1.(task_decl)) (task_hash t1.(task_prev)).
+Definition tag (i: CoqBigInt.t) (t1: t) : t :=
+  {| task_decl := t1.(task_decl);
+     task_prev := t1.(task_prev);
+     task_known := t1.(task_known);
+     task_clone := t1.(task_clone);
+     task_meta := t1.(task_meta);
+     task_tag := CoqWeakhtbl.create_tag i |}. (*TODO: coq-record-update?*)
+End TaskHash.
+
+Module Hstask := hashcons.Make TaskHash.
+Definition mk_task (decl: tdecl_c) (prev: task) (known: known_map)
+  (clone: clone_map) (meta: meta_map) : hashcons_st task_hd task :=
+  (t <- (Hstask.hashcons {|
+    task_decl := decl;
+    task_prev := prev;
+    task_known := known;
+    task_clone := clone;
+    task_meta := meta;
+    task_tag := CoqWeakhtbl.dummy_tag
+  |});;
+  st_ret (Some t))%state.
+
+(* Constructors with Checks*)
